\SSbreak\\
\emph{Source: NYCMT, 2020 P9 of 10}\\
\emph{Proposer: \Pnjoy}\\
\emph{Problem ID: 138}\\
\emph{Date: 2021-02-20}\\
\SSbreak

\SSpsetQ{
Let \( p = 2053 \) be a prime. For positive integers \( x\) let 
\[ f(x) = x^{400} + x^{326} + x^{200} + x^{126} + 2\]
and let \( g(x)\) denote the unique integer \(0\leq y \leq p-1\) such that \( y^{1759} - x \) is divisible by \( p\). Compute the remainder when 
\[ \sum_{i=1}^{2052} g(f(i)) \] 
is divided by 2053. 
}\bigskip

\begin{solution}\hfil\medskip

    To find $y$, we want to raise $y^{1759} \equiv x \pmod{p}$ to a power $k$ such that $1759k \equiv 1 \pmod{p - 1}$; solving we get $k \equiv 7 \pmod{p - 1}$
    and so $y \equiv x^7 \pmod{p}$. It remains to sum $f(i)^7 \pmod{p}$. Since $g, g^2, \cdots , g^{p - 1}$ where $g$ is a generator is a permutation of the nonzero residues mod $p$
    we find that $$\sum_{i = 1}^{p - 1} i^k = \sum_{i = 1}^{p - 1} g^{ik} = g^k \left(\dfrac{g^{(p - 1)k} - 1}{g^k - 1}\right) \equiv 0 \pmod{p}$$ unless $p - 1 | k$
    in which case each of the $p - 1$ terms is $1$ for a sum of $-1 \pmod{p}$. Since the maximum coefficient in $f(x)^7$ is $7 \cdot 400 = 2800$ it suffices to
    find the coefficient of $x^{2052}$ and the constant term. Using multinomial expansion, this is equivalent to finding nonnegative integers $(a, b, c, d, e)$ 
    such that $400a + 326b + 200c + 126d + 0e = 2052 \iff 200a + 163b + 100c + 63d = 1026$ and $a + b + c + d + e = 7$. Notice $a > 1$ since $200 \cdot 1 + 163 \cdot 6 < 1026$ and 
    $a < 5$ since $200 \cdot 5 = 1000$ and no combination of $160, 100, 63$ will make that sum to $1026$. Also, reducing mod 9 yields $2a + b + c \equiv 0 \pmod{9} \iff a + 7 \equiv d + e \pmod{9}.$
    When $a = 2$, we are forced $d, e = 0$ so $163b + 100c = 626 \iff (a, b, c, d, e) = (2, 2, 3, 0, 0)$.
    When $a = 3$, we are forced $d = 0, 1$ so either $163b + 100c = 426, 363 \iff (a, b, c, d, e) = (3, 2, 1, 0, 1), (3, 1, 2, 1, 0)$.
    When $a = 4$, we have $163b + 100c + 63d = 226 \iff (a, b, c, d, e) = (4, 1, 0, 1, 1), (4, 0, 1, 2, 0)$.
    Remembering the constant term is $2^7$, it remains to sum 
    $$-\dbinom{7}{2, 2, 3, 0, 0} - 2\dbinom{7}{3, 2, 1, 0, 1} - \dbinom{7}{3, 1, 2, 1, 0} - 2\dbinom{7}{4, 1, 0, 1, 1} - \dbinom{7}{4, 0, 1, 2, 0} - 2^7 \equiv \boxed{1983} \pmod{2053}.$$
\end{solution}\bigskip
